Clean/Air/OrderedChannel.lean
@@ -194,8 +194,6 @@ def PartialBalancedChannel [DecidableEq F] (tables : Tables F) (channel : RawCha
     ∃ extraInteractions : List (Interaction F),
       -- the total of known + unknown interactions is balanced
       BalancedInteractions (tables.interactionsWith channel ++ extraInteractions) ∧
-      -- guarantee-side interactions are either active pulls or disabled padding
-      InteractionsWellFormed (tables.interactionsWith channel ++ extraInteractions) ∧
       -- the extra interactions are with the same channel.
       (∀ i ∈ extraInteractions, i.channel = channel) ∧
     -- additionally, we _assume_ that either the requirements on future interactions hold unconditionally,
@@ -208,11 +206,10 @@ def PartialBalancedChannel [DecidableEq F] (tables : Tables F) (channel : RawCha
 /-- Partial balance is trivially weaker than balance -/
 lemma partialBalancedChannel_of_balancedInteractions [DecidableEq F] {tables : Tables F} {channel : RawChannel F} :
     BalancedInteractions (tables.interactionsWith channel) →
-    InteractionsWellFormed (tables.interactionsWith channel) →
     PartialBalancedChannel tables channel := by
-  intro balanced wellformed
+  intro balanced
   use []
-  simp [balanced, wellformed]
+  simp [balanced]
 
 /--
 For ordered channels, we can always instantiate partial balance at an initial sublist.
@@ -224,15 +221,12 @@ theorem partialBalancedChannel_of_cons_of_orderedChannelLt [DecidableEq F]
   PartialBalancedChannel (.cons table tables same_data) channel →
   OrderedChannelLt channel tables.components [table.component] →
     PartialBalancedChannel tables channel := by
-  rintro table_constraints ⟨ extraInteractions, balanced, wellformed, same_channel, extra_reqs_or_no_grts ⟩ not_in_reqs_or
+  rintro table_constraints ⟨ extraInteractions, balanced, same_channel, extra_reqs_or_no_grts ⟩ not_in_reqs_or
   use table.interactionsWith channel ++ extraInteractions
   simp only [circuit_norm] at *
   simp [or_imp] at ⊢ not_in_reqs_or extra_reqs_or_no_grts
   constructor
   · apply balancedInteractions_of_perm balanced
-    grw [List.perm_append_comm_assoc]
-  constructor
-  · apply wellformed.of_perm
     grw [List.perm_append_comm_assoc]
   constructor
   · intro a
@@ -289,7 +283,7 @@ lemma guarantees_of_requirements_cons [DecidableEq F]
   · exact table.guarantees_of_not_mem grts
   replace reqs := table.requirements_of_not_mem table_constraints reqs
   -- there's a special case to discard where the guarantees are trivially satisfied
-  rcases partial_balance with ⟨ extraInteractions, balanced, wellformed, same_channel, grts | extra_reqs ⟩
+  rcases partial_balance with ⟨ extraInteractions, balanced, same_channel, grts | extra_reqs ⟩
   · simp only [circuit_norm] at grts
     exact table.guarantees_of_not_mem grts.left
   -- now, to prove this table's channel guarantees, we show guarantees on _all_ channel interactions (that we know are balanced)
@@ -319,7 +313,7 @@ lemma guarantees_of_requirements_cons [DecidableEq F]
     · exact ⟨ same_channel i h_mem_extra, extra_reqs i h_mem_extra ⟩
   -- consistent channels goes from requirements to guarantees
   -- uses `consistent_channels` and `partial_balance`
-  apply ‹channel.Consistent›.consistent channelInteractions tables.data balanced wellformed all_reqs
+  apply ‹channel.Consistent›.consistent channelInteractions tables.data balanced all_reqs
 
 /--
 Partial balance can be specialized to a sublist (= part of a permutation),
@@ -331,12 +325,12 @@ lemma partialBalancedChannel_of_sublist [DecidableEq F] {subtables tables : Tabl
     (∀ table ∈ otherTables, table.Constraints) ∧
     ∀ table ∈ otherTables, channel ∉ table.channelsWithRequirements) →
     PartialBalancedChannel subtables channel := by
-  rintro ⟨ extraInteractions, balanced, wellformed, same_channel, no_grts_or_extra_reqs ⟩ subset_tables
+  rintro ⟨ extraInteractions, balanced, same_channel, no_grts_or_extra_reqs ⟩ subset_tables
   obtain ⟨ otherTables, perm, otherConstraints, otherReqs ⟩ := subset_tables
   by_cases subtables_empty : subtables.tables = []
   · simp [subtables_empty, circuit_norm, PartialBalancedChannel, Tables.interactionsWith]
     use []
-    simp [BalancedInteractions, balanceOf, InteractionsWellFormed]
+    simp [BalancedInteractions, balanceOf]
     by_cases h : ringChar F = 0
     · exact Or.inr h
     · exact Or.inl (Nat.pos_of_ne_zero h)
@@ -354,11 +348,6 @@ lemma partialBalancedChannel_of_sublist [DecidableEq F] {subtables tables : Tabl
   constructor; swap
   -- TODO this half is surprisingly long/annoying, maybe missing helper lemmas
   · simp [circuit_norm, or_imp]
-    constructor
-    · apply wellformed.of_perm
-      simp only [Tables.interactionsWith]
-      grw [← List.append_assoc, List.perm_append_right_iff, ← List.flatMap_append, perm.flatMap]
-      exact fun _ _ => List.Perm.refl _
     constructor
     · intro i
       use fun _ _ => Table.channel_eq_of_mem_interactionsWith
